src/program_proof/mvcc/txn_proof.v
@@ -715,24 +715,112 @@ Proof.
 Qed.
 
 (*****************************************************************)
+(* func (txnMgr *TxnMgr) getMinActiveTIDSite(sid uint64) uint64  *)
+(*****************************************************************)
+Theorem wp_txnMgr__getMinActiveTIDSite txnmgr sid γ :
+  is_txnmgr txnmgr γ -∗
+  {{{ True }}}
+    TxnMgr__getMinActiveTIDSite #txnmgr #sid
+  {{{ (tid : u64), RET #tid; site_min_tid_lb γ sid (int.nat tid) }}}.
+Proof.
+Admitted.
+
+(*****************************************************************)
 (* func (txnMgr *TxnMgr) getMinActiveTID() uint64                *)
 (*****************************************************************)
 Theorem wp_txnMgr__getMinActiveTID txnmgr γ :
+  is_txnmgr txnmgr γ -∗
   {{{ True }}}
-    TxnMgr__getMinActiveTID txnmgr
+    TxnMgr__getMinActiveTID #txnmgr
   {{{ (tid : u64), RET #tid; min_tid_lb γ (int.nat tid) }}}.
 Proof.
+  iIntros "#Htxnmgr" (Φ) "!> _ HΦ".
+  wp_call.
+  
   (***********************************************************)
   (* var min uint64 = config.TID_SENTINEL                    *)
+  (***********************************************************)
+  wp_apply (wp_ref_to); first auto.
+  iIntros (minRef) "HminRef".
+  wp_pures.
+    
+  (***********************************************************)
   (* for sid := uint64(0); sid < config.N_TXN_SITES; sid++ { *)
   (*     tid := txnMgr.getMinActiveTIDSite(sid)              *)
   (*     if tid < min {                                      *)
   (*         min = tid                                       *)
   (*     }                                                   *)
   (* }                                                       *)
+  (***********************************************************)
+  wp_apply (wp_ref_to); first auto.
+  iIntros (sidRef) "HsidRef".
+  wp_pures.
+  set P := λ (i : u64), (∃ (tidmin : u64),
+    "HminRef" ∷ minRef ↦[uint64T] #tidmin ∗
+    "Htidlbs" ∷ [∗ list] sid ∈ (take (int.nat i) sids_all), site_min_tid_lb γ sid (int.nat tidmin))%I.
+  wp_apply (wp_forUpto P _ _ (U64 0) (U64 N_TXN_SITES) sidRef with "[] [HminRef HsidRef]"); first done.
+  { clear Φ.
+    iIntros (i Φ) "!> (Hloop & HsidRef & %Hbound) HΦ".
+    iNamed "Hloop".
+    wp_pures.
+    wp_load.
+    wp_apply (wp_txnMgr__getMinActiveTIDSite with "Htxnmgr").
+    iIntros (tid) "Htidlb".
+    wp_pures.
+    wp_load.
+    wp_pures.
+
+    wp_if_destruct.
+    - (* Find new min. *)
+      wp_store.
+      iApply "HΦ".
+      iModIntro.
+      iFrame.
+      iExists _.
+      iFrame.
+      replace (int.nat (word.add _ _)) with (S (int.nat i)); last by word.
+      rewrite (take_S_r _ _ i); last by apply sids_all_lookup.
+      iApply big_sepL_app.
+      iSplitL "Htidlbs".
+      { iApply (big_sepL_impl with "Htidlbs").
+        iModIntro.
+        iIntros (iN sid) "Hlookup Htidlb".
+        iApply (site_min_tid_lb_weaken with "Htidlb").
+        word.
+      }
+      { simpl. auto. }
+    - (* Same min. *)
+      iApply "HΦ".
+      iModIntro.
+      iFrame.
+      iExists _.
+      iFrame.
+      replace (int.nat (word.add _ _)) with (S (int.nat i)); last by word.
+      rewrite (take_S_r _ _ i); last by apply sids_all_lookup.
+      iApply big_sepL_app.
+      iSplitL "Htidlbs"; first done.
+      simpl.
+      iSplit; last done.
+      iApply (site_min_tid_lb_weaken with "Htidlb").
+      word.
+  }
+  { iFrame.
+    iExists _.
+    iFrame.
+    replace (int.nat 0) with 0%nat; last word.
+    rewrite take_0.
+    auto.
+  }
+  iIntros "[Hloop HsidRef]".
+  iNamed "Hloop".
+  wp_pures.
+  
+  (***********************************************************)
   (* return min                                              *)
   (***********************************************************)
-Admitted.
+  wp_load.
+  by iApply "HΦ".
+Qed.
 
 (*****************************************************************)
 (* func (txn *Txn) Begin()                                       *)
